unifying kernel launches and interfaces, not great yet

include/kuiper.h
@@ -38,17 +38,8 @@ void __MUST(cudaError_t rc, const char * str, const char *fname, int line)
 		__MUST(cudaGetLastError(), "kcall", __FILE__, __LINE__);	\
 	} while (0)
 
-#define KPR_KCALL_SHMEM(foo, nblk, nthr, e_size, cnt, ...)			\
-	do {									\
-		KPR_KCALL_SHMEM_ASYNC(foo, nblk, nthr, e_size, cnt, __VA_ARGS__);\
-		__MUST(cudaDeviceSynchronize(), "kcall", __FILE__, __LINE__);	\
-	} while(0)
-
 #define KPR_KCALL_ASYNC(foo, nblk, nthr, ...)					\
 	KPR_KCALL_SHMEM_ASYNC(foo, nblk, nthr, 0, 0, __VA_ARGS__)
-
-#define KPR_KCALL(foo, nblk, nthr, ...)					\
-	KPR_KCALL_SHMEM(foo, nblk, nthr, 0, 0, __VA_ARGS__)
 
 #define KPR_SHMEM()							\
 	({								\
