src/lib/kuiper/Kuiper.Kernel.Base.fsti
@@ -1,0 +1,86 @@
+module Kuiper.Kernel.Base
+#lang-pulse
+
+open Kuiper.Common
+open Pulse.Lib.Core
+open FStar.Ghost
+open Pulse.Lib.BigStar
+open Kuiper.ForEvery
+open Kuiper.IntAliases
+open Kuiper.Array
+open Kuiper.Base
+open Kuiper.Epoch
+open Kuiper.SizeT
+module SZ = FStar.SizeT
+open Pulse.Lib.Pledge
+
+val shmem_tok
+  (#a:Type u#0)
+  {| Kuiper.Sized.sized a |}
+  (#sz:nat)
+  (ar:gpu_array a sz)
+: slprop
+
+(* This is the single primitive for launching kernels, with the most general
+type and capabilities. There are many simpler versions in the Kuiper.Kernel module,
+all implemented using this one and without any extra assumptions. *)
+fn launch_kernel_n_m_shmem_async
+  (nblk : szp { nblk <= max_blocks })
+  (nthr : szp { nthr <= max_threads })
+  (#pre #post : natlt nblk -> natlt nthr -> slprop)
+  (a : Type u#0) {| Kuiper.Sized.sized a |}
+  (smem_sz : SZ.t)
+  (#shared_pre #shared_post : gpu_array a smem_sz -> natlt nblk -> natlt nthr -> slprop)
+  (setup :
+    (ar: gpu_array a smem_sz) ->
+    (bid: natlt nblk) ->
+    stt_ghost unit emp_inames
+      (block_setup nthr ** (exists* v. gpu_pts_to_array #a #smem_sz ar #1.0R v))
+      (fun _ -> block_setup nthr ** bigstar 0 nthr (shared_pre ar bid)))
+  (k :
+    (ar: erased (gpu_array a smem_sz)) ->
+    (etid: tid_t { gdim_x etid == nblk /\ bdim_x etid == nthr }) ->
+    stt unit
+      (         gpu **
+                thread_id etid **
+                shmem_tok ar **
+                shared_pre ar (bidx_x etid) (tidx_x etid) **
+                pre (bidx_x etid) (tidx_x etid))
+      (fun _ -> gpu **
+                thread_id etid **
+                // shmem_tok ar **
+                shared_post ar (bidx_x etid) (tidx_x etid) **
+                post (bidx_x etid) (tidx_x etid))
+  )
+  (#e : epoch_t)
+  requires
+    cpu **
+    epoch_live e **
+    (forall+ (b : natlt nblk) (t : natlt nthr). pre b t)
+  returns
+    e' : epoch_t
+  ensures
+    cpu **
+    epoch_live e' **
+    pledge0 (epoch_done e')
+      (forall+ (b : natlt nblk) (t : natlt nthr). post b t) **
+    pure (e' >= e)
+
+fn obtain_shmem
+  (#a:Type u#0)
+  {| Kuiper.Sized.sized a |}
+  (#sz : erased nat)
+  (ear : erased (gpu_array a sz))
+  requires shmem_tok ear
+  returns  ar : gpu_array a sz
+  ensures  pure (reveal ear == ar)
+
+fn sync () (#e:epoch_t)
+  requires
+    epoch_live e
+  returns
+    e' : epoch_t
+  ensures
+    epoch_done e **
+    epoch_live e' **
+    pure (e' >= e)
